CoqOfRust/_std/cmp.v
@@ -1,3 +1,4 @@
+Require Import CoqOfRust.Monad.
 Require Import CoqOfRust.lib.lib.
 
 Require Import CoqOfRust._std.option.
@@ -35,14 +36,14 @@ Module PartialEq.
   Class Trait (Self : Set) (Rhs : option Set) : Set := {
     Rhs := defaultType Rhs Self;
 
-    eq : ref Self -> ref Rhs -> bool;
-    ne : ref Self -> ref Rhs -> bool;
+    eq : ref Self -> ref Rhs -> M bool;
+    ne : ref Self -> ref Rhs -> M bool;
   }.
 
-  Global Instance Method_eq `(Trait) : Notation.Dot "eq" := { 
+  Global Instance Method_eq `(Trait) : Notation.Dot "eq" := {
     Notation.dot := eq;
   }.
-  Global Instance Method_ne `(Trait) : Notation.Dot "ne" := { 
+  Global Instance Method_ne `(Trait) : Notation.Dot "ne" := {
     Notation.dot := ne;
   }.
 End PartialEq.
@@ -51,26 +52,26 @@ Module PartialOrd.
   Class Trait (Self : Set) (Rhs : option Set) : Set := {
     Rhs := defaultType Rhs Self;
 
-    partial_cmp : ref Self -> ref Self -> Option (Ordering);
-    lt : ref Self -> ref Rhs -> bool;
-    le : ref Self -> ref Rhs -> bool;
-    gt : ref Self -> ref Rhs -> bool;
-    ge : ref Self -> ref Rhs -> bool;
+    partial_cmp : ref Self -> ref Self -> M (option (Ordering.t));
+    lt : ref Self -> ref Rhs -> M bool;
+    le : ref Self -> ref Rhs -> M bool;
+    gt : ref Self -> ref Rhs -> M bool;
+    ge : ref Self -> ref Rhs -> M bool;
   }.
 
-  Global Instance Method_partial_cmp `(Trait) : Notation.Dot "partial_cmp" := { 
+  Global Instance Method_partial_cmp `(Trait) : Notation.Dot "partial_cmp" := {
     Notation.dot := partial_cmp;
   }.
-  Global Instance Method_lt `(Trait) : Notation.Dot "lt" := { 
+  Global Instance Method_lt `(Trait) : Notation.Dot "lt" := {
     Notation.dot := lt;
   }.
-  Global Instance Method_le `(Trait) : Notation.Dot "le" := { 
+  Global Instance Method_le `(Trait) : Notation.Dot "le" := {
     Notation.dot := le;
   }.
-  Global Instance Method_gt `(Trait) : Notation.Dot "gt" := { 
+  Global Instance Method_gt `(Trait) : Notation.Dot "gt" := {
     Notation.dot := gt;
   }.
-  Global Instance Method_ge `(Trait) : Notation.Dot "ge" := { 
+  Global Instance Method_ge `(Trait) : Notation.Dot "ge" := {
     Notation.dot := ge;
   }.
 End PartialOrd.
